theories/SLFWPsem.v
@@ -58,256 +58,359 @@ Lemma wp_weakest : forall t H Q,
   H ==> wp t Q.
 Proof using. introv M. rewrite <- wp_equiv. applys M. Qed.
 
-(** As we prove further in this chapter, it is possible to
-    define a function [wp] satisfying [wp_equiv]. Formally: *)
-
-Definition wp_characterization (wp:trm->(val->hprop)->hprop) :=
-  forall t H Q, (triple t H Q) <-> (H ==> wp t Q).
-
-Parameter wp_characterization_exists : exists wp0,
-  wp_characterization wp0.
-
-(** In fact, there are several ways in which [wp] can be defined.
-    It turns out that all possible definitions are equivalent.
-    In other words, the property captured by [wp_characterization]
-    defines a unique function. We next formally justify this fact. *)
-
-Lemma wp_characterization_unique : forall wp1 wp2,
-  wp_characterization wp1 ->
-  wp_characterization wp2 ->
-  wp1 = wp2.
-Proof using.
-  asserts L: (forall t Q wp1 wp2,
-    wp_characterization wp1 ->
-    wp_characterization wp2 ->
-    wp1 t Q ==> wp2 t Q).
-  { introv M1 M2. unfolds wp_characterization.
-    rewrite <- M2. rewrite M1. applys himpl_refl. }
-  introv M1 M2. applys fun_ext_2. intros t Q.
-  applys himpl_antisym; applys L; auto.
-Qed.
-
-(** Thus, it really does not matter which definition of [wp] is
-    considered. Thereafter, we only exploit the characterization lemma
-    [wp_equiv], and never rely on the internal definition of [wp]. *)
+(** There are several ways to define [wp]. It turns out that all
+    definitions are provably equivalent. In other words, the 
+    equivalence [(triple t H Q) <-> (H ==> wp t Q)] characterizes
+    a unique predicate [wp]. 
+    
+    The details of the possible direct definitions for [wp] are 
+    irrelevant to the main focus of this chapter, hence we postpone
+    the related discussion to the appendix. *)
 
 
 (* ******************************************************* *)
-(** ** Structural properties of weakest preconditions *)
+(** ** Structural rules in weakest-precondition style *)
 
-(** It is interesting to observe how the structural rules
-    can be applied on a judgment of the form [H ==> wp t Q].
-
-    At this stage, we'll make three important observations.
-
-    1. The extraction rules [triple_hexists] and [triple_hpure]
-       are not needed in a wp-style presentation, because they
-       are directly subsumed by basic lemmas on entailment.
-
-    2. The combined consequence-frame rule for [triple]
-       has a counterpart for [wp]. This rule is, in effect,
-       the unique structural rule that is needed for [wp].
-       (All other structural rules are derivable from it.)
-
-    3. The ramified-frame rule for [triple] also has a
-       counterpart for [wp]. This ramified rule for [wp]
-       will play a crucial rule in the construction of the function
-       that computes weakest precondition in the next chapter. *)
+(** We next discuss formulations of the frame rule and of the rule
+    of consequence in weakest-precondition style. *)
 
 
 (* ------------------------------------------------------- *)
-(** *** 1. Extraction rules are no longer needed *)
+(** *** The frame rule *)
 
-(** Recall the extraction rule for existentials: *)
+(** The frame rule for [wp] asserts that [(wp t Q) \* H] entails 
+    [wp t (Q \*+ H)]. This statement can be read as follows: 
+    if you own both a piece of state satisfying [H] and a piece of state 
+    in which the execution of [t] produces [Q], then you own a piece 
+    of state in which the execution of [t] produces [Q \*+ H], that is,
+    produces both [Q] and [H]. *)
 
-Parameter triple_hexists : forall t (A:Type) (J:A->hprop) Q,
-  (forall x, triple t (J x) Q) ->
-  triple t (\exists x, J x) Q.
+Lemma wp_frame : forall t H Q,
+  (wp t Q) \* H ==> wp t (Q \*+ H).
 
-(** Replacing [triple t H Q] with [H ==> wp t Q] yields: *)
+(** The lemma is proved by exploiting the frame rule for triples
+    and the equivalence that characterizes [wp]. *)
 
-Lemma triple_hexists_in_wp : forall t Q A (J:A->hprop),
-  (forall x, (J x ==> wp t Q)) ->
-  (\exists x, J x) ==> wp t Q.
-
-(** This implication is just a special case of the lemma
-    [himpl_hexists_l], which proves [(\exists x, J x) ==> H]
-    from [forall x, (J x ==> H)]. *)
-
-Proof using. introv M. applys himpl_hexists_l M. Qed.
-
-(** In other words, in the [wp] presentation, we don't need
-    a specific extraction rule for existentials, because the
-    extraction rule for entailment already does the job. *)
-
-(** Likewise for [triple_hpure], which enables extracting pure
-    facts from precondition: the rule [himpl_hstar_hpure_l] may be
-    used to prove [\[P] \* H1 ==> H2] from [\[P] -> H1 ==> H2]. *)
-
-
-(* ------------------------------------------------------- *)
-(** *** 2. Combined structural rule for [wp] *)
-
-(** Recall the combined consequence-frame rule for [triple]. *)
-
-Parameter triple_conseq_frame : forall H2 H1 Q1 t H Q,
-  triple t H1 Q1 ->
-  H ==> H1 \* H2 ->
-  Q1 \*+ H2 ===> Q ->
-  triple t H Q.
-
-(** Let us reformulate this rule using [wp]:
-
-[[
-    H1 ==> wp t Q1 ->
-    H ==> H1 \* H2 ->
-    Q1 \*+ H2 ===> Q ->
-    H ==> wp t Q.
-]]
-
-   The beove statement can be simplified by substituting [H]
-   with [H1 \* H2], then substituting [H1] with [wp t Q1].
-   We obtain:
-
-[[
-    Q1 \*+ H2 ===> Q ->
-    (wp t Q1) \* H2 ==> wp t Q.
-]]
-   After renaming [H2] into [H] and [Q] into [Q2], we arrive at
-   the combined rule for [wp]:
-*)
-
-Lemma wp_conseq_frame : forall t H Q1 Q2,
-  Q1 \*+ H ===> Q2 ->
-  (wp t Q1) \* H ==> (wp t Q2).
 Proof using.
-  introv M. rewrite <- wp_equiv.
-  applys triple_conseq_frame (wp t Q1) M.
-  { rewrite wp_equiv. xsimpl. } { xsimpl. }
+  intros. rewrite <- wp_equiv.
+  applys triple_frame. rewrite~ wp_equiv.
 Qed.
 
-(** The above statement asserts that:
+(** The connection with the frame is not be totally obvious.
+    Recall the frame rule for triples.
 
-    1. [wp t Q1] can absorb any heap predicate [H] with which it
-      is starred, changing it to [wp t (Q1 \*+ H)].
+[[
+    triple t H1 Q ->
+    triple t (H1 \* H) (Q \*+ H)
+]]
+    Let us replace the form [triple t H Q] with the form
+    [H ==> wp t Q]. We obtain the following statement: *)
 
-    2. [wp t Q1] can be weakened to [wp t Q2] when [Q1 ===> Q2]. *)
+Lemma wp_frame_trans : forall t H1 Q H,
+  H1 ==> wp t Q ->
+  (H1 \* H) ==> wp t (Q \*+ H).
 
-(** Further in this chapter, we present specializations of
-    this rule, e.g., to invoke only the [frame] rule, or only the
-    garbage collection rule. *)
+(** If we exploit transitivity to eliminate [H1], we obtain 
+    exactly [wp_frame]. *)
+
+Proof using. introv M. xchange M. applys* wp_frame. Qed.
 
 
 (* ------------------------------------------------------- *)
-(** *** 3. The ramified structural rule for [wp] *)
+(** *** The rule of consequence *)
 
-(** Consider the entailment [Q1 \*+ H ===> Q2]
-    that appears in the combined rule [wp_conseq_frame].
+(** The rule of consequence for [wp] materializes as a covariance
+    property: asserting that [wp t Q] is covariante in [Q].
+    In other words, if one weakens [Q] then one weakens [wp t Q].
+    Formally: *)
 
-    This entailement can be rewritten using the magic wand as:
-    [H ==> (Q1 \--* Q2)].
+Lemma wp_conseq : forall t Q1 Q2,
+  Q1 ===> Q2 ->
+  wp t Q1 ==> wp t Q2.
+Proof using.
+  introv M. rewrite <- wp_equiv. applys~ triple_conseq (wp t Q1) M. applys wp_pre. 
+Qed.
 
-    Thus, the conclusion [(wp t Q1) \* H ==> (wp t Q2)]
-    can be reformulated as
-    [(wp t Q1) \* (Q1 \--* Q2) ==> (wp t Q2)].
+(** The connection with the rule of consequence is, again, not so obvious.
+    Recall the rule of consequence.
 
-    The "ramified combined structural rule" for [wp], shown below,
-    captures in a single line all the structural properties of [wp]. *)
+[[
+    triple t H1 Q1 ->
+    H2 ==> H1 ->
+    Q1 ===> Q2 ->
+    triple t H2 Q2
+]]
+    Let us replace the form [triple t H Q] with the form [H ==> wp t Q].
+    We obtain the following statement: *)
 
-Lemma wp_ramified : forall t Q1 Q2,
-  (wp t Q1) \* (Q1 \--* Q2) ==> (wp t Q2).
-Proof using. intros. applys wp_conseq_frame. xsimpl. Qed.
+Lemma wp_conseq_trans : forall t H1 H2 Q1 Q2,
+  H1 ==> wp t Q1 ->
+  H2 ==> H1 ->
+  Q1 ===> Q2 ->
+  H2 ==> wp t Q2.
 
-(** The following specialization is useful to apply only frame. *)
+(** As we prove, this result is a corrolary [wp_conseq] and
+    transitivity of entailement. *)
 
-Lemma wp_ramified_frame : forall t Q1 Q2,
-  (wp t Q1) \* (Q1 \--* Q2) ==> (wp t Q2).
-Proof using. intros. applys wp_conseq_frame. xsimpl. Qed.
+Proof using. 
+  introv M WH WQ. xchanges WH. xchanges M. applys wp_conseq WQ.
+Qed.
 
-(** The following reformulation is handy to apply on any goal
-    of the form [H ==> wp t Q]. *)
 
-Lemma wp_ramified_trans : forall t H Q1 Q2,
-  H ==> (wp t Q1) \* (Q1 \--* Q2) ->
-  H ==> (wp t Q2).
-Proof using. introv M. xchange M. applys wp_ramified. Qed.
+(* ------------------------------------------------------- *)
+(** *** The extraction rules *)
 
+(** The extraction rules [triple_hpure] and [triple_hexists]
+    have no specific counterpart with the [wp] presentation.
+    Indeed, these extraction rules are already captured by
+    the extraction rules for entailement. 
+
+    To see why, consider for example the rule [triple_hpure]. *)
+
+Parameter triple_hpure : forall t (P:Prop) H Q,
+  (P -> triple t H Q) ->
+  triple t (\[P] \* H) Q.
+
+(** Replacing the form [triple t H Q] with [H ==> wp t Q] yields: *)
+
+Lemma triple_hpure_with_wp : forall t H Q (P:Prop),
+  (P -> (H ==> wp t Q)) ->
+  (\[P] \* H) ==> wp t Q.
+
+(** The above implication is just a special case of the extraction
+    lemma for pure facts on the left on an entailment, named
+    [himpl_hstar_hpure_l], which asserts:
+[[
+  (P -> H ==> H') ->
+  (\[P] \* H) ==> H'.
+]]  
+    Indeed:
+*)
+
+Proof using. introv M. applys himpl_hstar_hpure_l M. Qed.
+
+(** A similar reasoning applies to the extraction rule for existentials. *)
+
+
+(* ******************************************************* *)
+(** ** Reasoning rules for terms, in weakest-precondition style *)
+
+(* ------------------------------------------------------- *)
+(** *** Rules for values *)
+
+(** Recall the rule [triple_val] which gives a reasoning rule for
+    establishing a triple for a value [v]. *)
+
+Parameter triple_val : forall v H Q,
+  H ==> Q v ->
+  triple (trm_val v) H Q.
+
+(** If we rewrite this rule in [wp] style, we obtain:
+[[
+    H ==> Q v ->
+    H ==> wp (trm_val v) Q.
+]]
+    By exploiting transitivity of entailment, we can eliminate [H].
+    We obtain the following statement, which reads as follows:
+    if you own a state satisfying [Q v], then you own a state 
+    from which the evaluation of the value [v] satisfies the
+    postcondition [Q].
+*)
+
+Lemma wp_val : forall v Q,
+  Q v ==> wp (trm_val v) Q.
+Proof using.
+  intros. rewrite <- wp_equiv. applys* triple_val.
+Qed.
+
+(** Let us verify that while migrating to the [wp] presentation we have
+    not lost any expressivity, by showing that from [wp_val] we are able
+    to recover [triple_val]. *)
+
+Lemma triple_val_derived_from_wp_val : forall v H Q,
+  H ==> Q v ->
+  triple (trm_val v) H Q.
+Proof using. introv M. rewrite wp_equiv. xchange M. applys wp_val. Qed.
+
+
+(* ------------------------------------------------------- *)
+(** *** Rules for sequence *)
+
+(** Recall the reasoning rule for a sequence [trm_seq t1 t2]. *)
+
+Parameter triple_seq : forall t1 t2 H Q H1,
+  triple t1 H (fun v => H1) ->
+  triple t2 H1 Q ->
+  triple (trm_seq t1 t2) H Q.
+
+(** Replacing [triple t H Q] with [H ==> wp t Q] throughout the rule gives:
+
+[[
+      H ==> (wp t1) (fun v => H1) ->
+      H1 ==> (wp t2) Q ->
+      H ==> wp (trm_seq t1 t2) Q.
+]]
+    This entailment holds for any [H] and [H1]. Let us specialize it to
+    [H1 := (wp t2) Q] and [H := (wp t1) (fun v => (wp t2) Q)].
+
+    This leads us to the following statement, which reads as follows:
+    if you own a state from which the evaluation of [t1] 
+    produces a state from which the evaluation of [t2]
+    produces the postcondition [Q], then you own a state from
+    which the evaluation of the sequence [t1;t2] produces [Q]. *)
+
+Lemma wp_seq : forall t1 t2 Q,
+  wp t1 (fun r => wp t2 Q) ==> wp (trm_seq t1 t2) Q.
+Proof using.
+  intros. rewrite <- wp_equiv. applys triple_seq.
+  { rewrite~ wp_equiv. }
+  { rewrite~ wp_equiv. }
+Qed.
+
+(* EX2! (triple_seq_from_wp_seq) *)
+(** Check that [wp_seq] is just as expressive as [triple_seq],
+    by proving that [triple_seq] is derivable from [wp_seq]
+    and from the structural rules for [wp] and/or the structural
+    rules for [triple]. *)
+
+Lemma triple_seq_from_wp_seq : forall t1 t2 H Q H1,
+  triple t1 H (fun v => H1) ->
+  triple t2 H1 Q ->
+  triple (trm_seq t1 t2) H Q.
+Proof using.
+(* SOLUTION *)
+  introv M1 M2. rewrite wp_equiv in *. xchange M1.
+  applys himpl_trans wp_seq. applys wp_conseq. intros _. applys M2.
+(* /SOLUTION *)
+Qed.
 
 
 (* ####################################################### *)
-(** * Realization of [wp], and structural properties *)
+(** * Additional contents *)
 
 (* ******************************************************* *)
-(** ** Semantic definition of weakest precondition *)
+(** ** Other reasoning rules for terms *)
 
-(** The lemma [wp_equiv] asserts [(triple t H Q) <-> (H ==> wp t Q)].
-    We have seen in the introduction of this chapter that [wp_equiv]
-    defines a unique function [wp]. There remains to show that there
-    actually exists at least one such function.
+(* ------------------------------------------------------- *)
+(** *** Rule for functions *)
 
-    Recall the definition of [wp_characterization].
+(** Recall the reasoning rule for a term [trm_fun x t1],
+    which evaluates to the value [val_fun x t1]. *)
+
+Parameter triple_fun : forall x t1 H Q,
+  H ==> Q (val_fun x t1) ->
+  triple (trm_fun x t1) H Q.
+
+(** The rule for functions follow exactly the same pattern as for values. *)
+
+Lemma wp_fun : forall x t Q,
+  Q (val_fun x t) ==> wp (trm_fun x t) Q.
+Proof using. intros. rewrite <- wp_equiv. applys* triple_fun. Qed.
+
+(** A similar rule holds for the evaluation of a recursive function. *)
+
+
+(* ------------------------------------------------------- *)
+(** *** Rule for conditionals *)
+
+(** Recall the reasoning rule for a term [triple_if b t1 t2]. *)
+
+Parameter triple_if_case : forall b t1 t2 H Q,
+  triple (if b then t1 else t2) H Q ->
+  triple (trm_if (val_bool b) t1 t2) H Q.
+
+(** Replacing [triple] using [wp] entailements yields:
+
 [[
-    Definition wp_characterization (wp:trm->(val->hprop)->hprop) :=
-      forall t H Q, (triple t H Q) <-> (H ==> wp t Q).
+    H ==> wp (if b then t1 else t2) Q ->
+    H ==> wp (trm_if (val_bool b) t1 t2) Q.
+]]
+    which simplifies by transitivity to:
+[[
+    wp (if b then t1 else t2) Q ==> wp (trm_if (val_bool b) t1 t2) Q.
 ]]
 *)
 
-(** In what follows, we'll give two possible definitions, a
-    low-level one expressed as a function on heaps, and a high-level
-    one expressed using only Separation Logic combinators.
-    For both, we'll show that they satisfy [wp_characterization].
-
-    Note that, by lemma [wp_characterization_unique], the two
-    definitions that we consider are necessarily equivalent to
-    each other. *)
-
-(** Firstly, we present the "low-level" definition of [wp t Q].
-    It is defined as a heap predicate that holds of a heap [h]
-    if and only if the execution of [t] starting the heap [h]
-    produces the post-condition [Q].
-
-    Technically, it is defined as [fun h => triple t (=h) Q], 
-    where [=h] is a shorthand for [fun h' => (h' = h)]. 
-    In other words, the precondition [=h] requires the input heap 
-    to be identical to [h]. *)
-
-Definition wp_low (t:trm) (Q:val->hprop) : hprop :=
-  fun (h:heap) => triple t (=h) Q.
-
-(** We next shot that [wp_low] statisfies the equivalence 
-    [triple t H Q <-> H ==> wp Q] that characterizes [wp]. *)
-
-Lemma wp_equiv_wp_low : wp_characterization wp_low.
-  (** [forall t H Q, (triple t H Q) <-> (H ==> wp_low t Q)]. *)
-Proof using.
-  (** This proof is a bit technical, it is not required to follow it.
-      It requires the lemma [triple_named_heap] established
-      as exercise in an earlier chapter. *)
-  unfold wp_low. iff M.
-  { intros h K. applys triple_conseq M.
-    { intros h' ->. applys K. }
-    { applys qimpl_refl. } }
-  { applys triple_named_heap. intros h K.
-    applys triple_conseq (=h) Q.
-    { specializes M K. applys M. }
-    { intros ? ->. auto. }
-    { applys qimpl_refl. } }
+Lemma wp_if : forall b t1 t2 Q,
+  wp (if b then t1 else t2) Q ==> wp (trm_if b t1 t2) Q.
+Proof using. 
+  intros. rewrite <- wp_equiv. applys triple_if.
+  { intros ->. rewrite~ wp_equiv. }
+  { intros ->. rewrite~ wp_equiv. }
 Qed.
 
-(** Secondly, we present the "high-level" definition of [wp t Q].
-    It is "higher-level" because it is defined using Separation Logic 
-    combinators, without resorting to the manipulation of heaps.
+
+(* ------------------------------------------------------- *)
+(** *** Rule for let-bindings *)
+
+(** Recall the reasoning rule for a term [trm_let x t1 t2]. *)
+
+Parameter triple_let : forall x t1 t2 H Q Q1,
+  triple t1 H Q1 ->
+  (forall v, triple (subst x v t2) (Q1 v) Q) ->
+  triple (trm_let x t1 t2) H Q.
+
+(** The rule of [trm_let x t1 t2] is very similar to that for
+    [trm_seq], the only difference being the substitution. *)
+
+Lemma wp_let : forall x t1 t2 Q,
+  wp t1 (fun v => wp (subst x v t2) Q) ==> wp (trm_let x t1 t2) Q.
+Proof using. 
+  intros. rewrite <- wp_equiv. applys triple_let.
+  { rewrite~ wp_equiv. }
+  { intros v. rewrite~ wp_equiv. }
+Qed.
+
+
+(* ------------------------------------------------------- *)
+(** *** Rule for function applications *)
+
+(** Recall the reasoning rule for an application [(val_fun x t1) v2]. *)
+
+Parameter triple_app_fun : forall x v1 v2 t1 H Q,
+  v1 = val_fun x t1 ->
+  triple (subst x v2 t1) H Q ->
+  triple (trm_app v1 v2) H Q.
+
+(** The corresponding [wp] rule is stated and proved next. *)
+
+Lemma wp_app_fun : forall x v1 v2 t1 Q,
+  v1 = val_fun x t1 ->
+  wp (subst x v2 t1) Q ==> wp (trm_app v1 v2) Q.
+Proof using.
+  introv EQ1. rewrite <- wp_equiv. applys* triple_app_fun.
+  rewrite~ wp_equiv.
+Qed.
+
+(** A similar rule holds for the application of a recursive function. *)
+
+
+(* ####################################################### *)
+(** * Bonus contents (optional reading) *)
+
+(* ******************************************************* *)
+(** ** A concrete definition for weakest precondition *)
+
+Module WpHighLevel.
+
+(** The lemma [wp_equiv] captures the characteristic property of [wp],
+    that is, [(triple t H Q) <-> (H ==> wp t Q)].
+
+    However, it does not give evidence that there exists a predicate [wp]
+    satisfying this equivalence. We next present one possible definition. 
 
     The idea is to define [wp t Q] as the predicate 
-    [\exists H, H \* \[triple t H Q]]. As we argue next,
-    this heap predicate is entailed by any valid precondition,
-    and it is itself a valid precondition.
-*)
+    [\exists H, H \* \[triple t H Q]].  *)
 
-Definition wp_high (t:trm) (Q:val->hprop) : hprop :=
+Definition wp (t:trm) (Q:val->hprop) : hprop :=
   \exists (H:hprop), H \* \[triple t H Q].
 
-(** On the one hand, if [H'] is a valid precondition, i.e. such that
+(** As we argue next, the heap predicate [wp t Q] is entailed by 
+    any precondition [H'] that satisfies [triple t H' Q],
+    and [wp t Q] is itself a valid precondition, in the sense that
+    [triple t (wp t Q) Q].
+
+    On the one hand, if [H'] is a valid precondition, i.e. such that
     [triple t H' Q] holds, then it is the case that 
     [H' ==> \exists H, H \* \[triple t H Q]].
     Indeed, the entailment holds by instantiating [H] as [H'].
@@ -325,14 +428,14 @@ Definition wp_high (t:trm) (Q:val->hprop) : hprop :=
     [triple t H Q <-> H ==> wp Q], which characterizes [wp]. *)
 
 (* EX2! (wp_equiv_wp_high) *)
-(** Prove that this second definition of [wp] statisfies
-    the characteristic property [wp_equiv]. *)
+(** Prove that the definition [wp_high] statisfies the characteristic
+    equivalence for weakest preconditions. *)
 
-Lemma wp_equiv_wp_high : wp_characterization wp_high.
-  (** [forall t H Q, (triple t H Q) <-> (H ==> wp_high t Q)]. *)
+Lemma wp_equiv_wp : forall t H Q,
+  (triple t H Q) <-> (H ==> wp t Q).
 Proof using.
 (* SOLUTION *)
-  unfold wp_characterization, wp_high. iff M.
+  unfold wp. iff M.
   { xsimpl H. apply M. }
   { applys triple_conseq Q M.
     { applys triple_hexists. intros H'.
@@ -342,408 +445,348 @@ Proof using.
 (* /SOLUTION *)
 Qed.
 
+(* TODO: problem, we give the same proof further in the file. *)
+
+End WpHighLevel.
+
 
 (* ******************************************************* *)
-(** ** Specialized versions of the structural rule for [wp] *)
+(** ** An alternative definition for weakest precondition *)
 
-(** The combined structural rule for [wp] captures all the
-    structural rules. We here discuss the formulation of
-    specializations of this rule. The corresponding lemmas
-    highlight interesting properties of the [wp] operator. *)
+Module WpLowLevel.
 
-(** One important property of [wp] is its covariance, which
-    corresponds to the rule of consequence for [wp]. It asserts
-    that [wp t Q] is covariante in [Q], as we state and prove next. *)
+(** The concrete definition for [wp] given above is expressed 
+    in terms of Separation Logic combinators. In constrast to
+    this "high level" definition, there exists a more "low level"
+    definition, expressed directly as a function over heaps.
 
-Lemma wp_conseq : forall t Q1 Q2,
-  Q1 ===> Q2 ->
-  wp t Q1 ==> wp t Q2.
-Proof using.
-  introv M. lets N: wp_ramified t Q1 Q2. xchanges N. xchanges M.
+    In that alternative definition, the heap predicate [wp t Q] 
+    is defined as a predicate that holds of a heap [h]
+    if and only if the execution of [t] starting in exactly
+    the heap [h]produces the post-condition [Q].
+
+    Technically, [wp t Q] is defined as [fun h => triple t (=h) Q],
+    where [=h] is a shorthand for [fun h' => (h' = h)].
+    In other words, the precondition [=h] requires the input heap
+    to be exactly [h]. *)
+
+Definition wp (t:trm) (Q:val->hprop) : hprop :=
+  fun (h:heap) => triple t (=h) Q.
+
+(** One can prove that this definition of [wp] also statisfies the
+    characteristic equivalence [triple t H Q <-> H ==> wp Q]. *)
+
+Lemma wp_equiv_wp_low : forall t H Q,
+  (triple t H Q) <-> (H ==> wp t Q).
+
+(** The details of the proofs are given for the reference but are
+    beyond the scope of this course. (The proof exploits the lemma
+    [triple_named_heap] which was established as an exercise in the
+    appendix of the chapter [SLFRules].) *)
+
+Proof using. (* Warning: details beyond the scope of the proof. *)
+  unfold wp. iff M.
+  { intros h K. applys triple_conseq M.
+    { intros h' ->. applys K. }
+    { applys qimpl_refl. } }
+  { applys triple_named_heap. intros h K.
+    applys triple_conseq (=h) Q.
+    { specializes M K. applys M. }
+    { intros ? ->. auto. }
+    { applys qimpl_refl. } }
 Qed.
 
-(** How can this rule simulate the rule of consequence, which also
-    enables strenthening the precondition? The following lemma
-    provides the answer: strenghtening of the precondition simply
-    consists of invoking the transitivy property of entailment. *)
+End WpLowLevel.
 
-Lemma wp_conseq_pre : forall t H' H Q,
-  H' ==> wp t Q ->
-  H ==> H' ->
+
+(* ******************************************************* *)
+(** ** Equivalence between all definitions of [wp] *)
+
+(** We next prove that the equivalence [(triple t H Q) <-> (H ==> wp t Q)]
+    defines a unique predicate [wp]. In other words, all possible 
+    definitions of [wp] are equivalent to each another.
+    Thus, it really does not matter which concrete definition
+    of [wp] we consider: they are all equivalent. 
+
+    Concretely, assume two predicates [wp1] and [wp2] to both satisfy
+    the caracteristic equivalence. We prove that they are equal. *)
+
+Lemma wp_unique : forall wp1 wp2,
+  (forall t H Q, (triple t H Q) <-> (H ==> wp1 t Q)) ->
+  (forall t H Q, (triple t H Q) <-> (H ==> wp2 t Q)) ->
+  wp1 = wp2.
+Proof using.
+  introv M1 M2. applys fun_ext_2. intros t Q. applys himpl_antisym.
+  { rewrite <- M2. rewrite M1. auto. }
+  { rewrite <- M1. rewrite M2. auto. }
+Qed.
+
+
+(* ******************************************************* *)
+(** ** Extraction rule for existentials *)
+
+(** Recall the extraction rule for existentials: *)
+
+Parameter triple_hexists : forall t (A:Type) (J:A->hprop) Q,
+  (forall x, triple t (J x) Q) ->
+  triple t (\exists x, J x) Q.
+
+(** Replacing [triple t H Q] with [H ==> wp t Q] yields the
+    following lemma. Prove it. *)
+
+(* EX2! (triple_hexists_in_wp) *)
+(** Prove the extraction rule for existentials in [wp] style. *)
+
+Lemma triple_hexists_in_wp : forall t Q A (J:A->hprop),
+  (forall x, (J x ==> wp t Q)) ->
+  (\exists x, J x) ==> wp t Q.
+
+Proof using. 
+  (* SOLUTION *)
+  introv M. applys himpl_hexists_l M. 
+  (* /SOLUTION *)
+Qed.
+
+(** In other words, in the [wp] presentation, we do not need
+    a specific extraction rule for existentials, because the
+    extraction rule for entailment already does the job. *)
+
+
+(* ******************************************************* *)
+(** ** Combined structural rule *)
+
+(** Recall the combined consequence-frame rule for [triple]. *)
+
+Parameter triple_conseq_frame : forall H2 H1 Q1 t H Q,
+  triple t H1 Q1 ->
+  H ==> H1 \* H2 ->
+  Q1 \*+ H2 ===> Q ->
+  triple t H Q.
+
+(** Let us reformulate this rule using [wp], replacing the
+    form [triple t H Q] with the form [H ==> wp t Q]. *)
+
+(* EX2? (wp_conseq_frame_trans) *)
+(** Prove the combined structural rule in [wp] style.
+    Hint: exploit [wp_conseq_trans] and [wp_frame]. *)
+
+Lemma wp_conseq_frame_trans : forall t H H1 H2 Q1 Q,
+  H1 ==> wp t Q1 ->
+  H ==> H1 \* H2 ->
+  Q1 \*+ H2 ===> Q ->
   H ==> wp t Q.
-Proof using. introv M WH. applys himpl_trans WH. applys M. Qed.
+Proof using. 
+  (* SOLUTION *)
+  introv M WH WQ. xchanges WH. xchange M.
+  applys wp_conseq_trans WQ. applys himpl_refl.
+  applys wp_frame.
+  (* /SOLUTION *)
+Qed.
 
-(** More generally, the consequence rule for goals in [wp] form
-    can be written in a form reminiscent of [triple_conseq]: *)
+(** The combined structural rule for [wp] can actually be stated
+    in a more concise way, as follows. *)
 
-Lemma wp_conseq_trans : forall t H' Q' H Q,
-  H' ==> wp t Q' ->
-  H ==> H' ->
-  Q' ===> Q ->
-  H ==> wp t Q.
-Proof using. introv M WH WQ. xchange WH. xchange M. applys wp_conseq WQ. Qed.
+(* EX2! (wp_conseq_frame) *)
+(** Prove the concise version of the combined structural rule 
+    in [wp] style. (Many proofs are possible.) *)
 
-(** Thereafter, we present rules in the form of entailments between [wp],
-    that is, [wp ... ==> wp ...], but keep in mind that this presentation
-    is equivalent to the form: [forall H, H ==> wp ... -> H ==> wp ...]. *)
-
-(** The frame rule for [wp] asserts that, given [(wp t Q) \* H],
-    the [wp] may absorb [H] and yield [(wp t (Q \*+ H)]. *)
-
-Lemma wp_frame : forall t H Q,
-  (wp t Q) \* H ==> wp t (Q \*+ H).
+Lemma wp_conseq_frame : forall t H Q1 Q2,
+  Q1 \*+ H ===> Q2 ->
+  (wp t Q1) \* H ==> (wp t Q2).
 Proof using.
-  intros. rewrite <- wp_equiv.
-  applys triple_frame. rewrite~ wp_equiv.
+  (* SOLUTION *)
+  dup 3.
+  { (* Proof using [wp_conseq_frame_trans] *)
+    introv M. applys* wp_conseq_frame_trans M. }
+  { (* Proof using [wp_frame] and [wp_conseq_trans] *)
+    introv M. applys~ wp_conseq_trans M. applys* wp_frame. }
+  { (* Proof using [triple_conseq_frame] *)
+    introv M. rewrite <- wp_equiv.
+    applys triple_conseq_frame (wp t Q1) M.
+    { rewrite wp_equiv. xsimpl. } { xsimpl. } }
+  (* /SOLUTION *)
 Qed.
 
 
-(* ####################################################### *)
-(** * Definition of [wp] directly in terms of [hoare] *)
-
 (* ******************************************************* *)
-(** ** Motivation for direct definitions for [wp] rules *)
+(** ** Alternative statement of the rule for conditionals *)
 
-(** In our construction, we have proved reasoning rules for
-    [hoare], derived reasoning rules for [triple], then used
-    the latter for proving the soundness of [wp].
+(** We have established the following rule for reasoning
+    about conditionals using [wp]. *)
 
-    Yet, if our goal was only to prove properties [wp], we wouldn't
-    need any result on [triple]. How would the reasoning rules be
-    stated and proved if we were to directly state and prove [wp]
-    properties from [hoare]? Let us investigate. *)
-
-(** We assume [wp] to be defined [wp] to be defined directly in terms
-    of [hoare], following the definition of [wp_high] from above. *)
-
-Parameter wp_def : forall t Q,
-  wp t Q = \exists H, H \* \[forall H', hoare t (H \* H') (Q \*+ H')].
-
-(** We first establish the (most-general) structural rule for [wp],
-    directly with respect to the [hoare] judgment. *)
-
-Lemma wp_ramified' : forall t Q1 Q2,
-  (wp t Q1) \* (Q1 \--* Q2) ==> (wp t Q2).
-Proof using.
-  intros. do 2 rewrite wp_def. xpull ;=> H M.
-  xsimpl (H \* (Q1 \--* Q2)). intros H'.
-  applys hoare_conseq M; xsimpl.
-Qed.
-
-(** We next establish [wp] reasoning rules for each term construct.
-
-    To guide us towards the appropriate statements, we start from the
-    rule for [triple], and reformulate it using the equivalence
-    [triple t H Q <-> H ==> (wp t Q)]. *)
-
-
-(* ******************************************************* *)
-(** ** Weakest precondition for values and functions *)
-
-(** First, consider a value [v]. Recall the rule [triple_val],
-    which asserts that [H ==> Q v] is a sufficient condition for
-    establishing [triple t (trm_val v) H Q]. *)
-
-Parameter triple_val : forall v H Q,
-  H ==> Q v ->
-  triple (trm_val v) H Q.
-
-(** Equivalently, [H ==> Q v] is a sufficient condition to establish
-    [H ==> wp (trm_val) Q]. Since this implication holds for any [H],
-    it holds in particular for [H := Q v]. Thus, the entailement
-    [Q v ==> wp (trm_val v) Q] holds. Let us formalize the statement,
-    then prove it directly in terms of the [hoare] reasoning rule for
-    values. *)
-
-Lemma wp_val : forall v Q,
-  Q v ==> wp (trm_val v) Q.
-Proof using. intros. rewrite wp_def. xsimpl; intros H'. applys hoare_val. xsimpl. Qed.
-
-(** Interestingly, we have not lost any expressive power: from [wp_val]
-    one can recover [triple_val]. *)
-
-Lemma triple_val_derived_from_wp_val : forall v H Q,
-  H ==> Q v ->
-  triple (trm_val v) H Q.
-Proof using. introv M. rewrite wp_equiv. xchange M. applys wp_val. Qed.
-
-(** The [wp] rules for [trm_fun] and [trm_fix] follow the exact same pattern. *)
-
-Lemma wp_fun : forall x t Q,
-  Q (val_fun x t) ==> wp (trm_fun x t) Q.
-Proof using. intros. rewrite wp_def. xsimpl; intros H'. applys hoare_fun. xsimpl. Qed.
-
-Lemma wp_fix : forall f x t Q,
-  Q (val_fix f x t) ==> wp (trm_fix f x t) Q.
-Proof using. intros. rewrite wp_def. xsimpl; intros H'. applys hoare_fix. xsimpl. Qed.
-
-
-(* ******************************************************* *)
-(** ** Weakest precondition for conditionals *)
-
-(** Consider a term [triple_if b t1 t2]. Recall the reasoning rule. *)
-
-Parameter triple_if_case : forall b t1 t2 H Q,
-  triple (if b then t1 else t2) H Q ->
-  triple (trm_if (val_bool b) t1 t2) H Q.
-
-(** Replacing [triple] using [wp] entailements yields:
-
-[[
-    H ==> wp (if b then t1 else t2) Q ->
-    H ==> wp (trm_if (val_bool b) t1 t2) Q.
-]]
-    which simplifies to:
-[[
-    wp (if b then t1 else t2) Q ==> wp (trm_if (val_bool b) t1 t2) Q.
-]]
-    This suggests.
-*)
-
-Lemma wp_if : forall b t1 t2 Q,
+Parameter wp_if' : forall b t1 t2 Q,
   wp (if b then t1 else t2) Q ==> wp (trm_if b t1 t2) Q.
-Proof using.
-  intros. repeat rewrite wp_def. xsimpl; intros H M H'.
-  applys hoare_if_case. applys M.
-Qed.
 
 (** Equivalently, the rule may be stated with the conditional around
     the calls to [wp t1 Q] and [wp t2 Q]. *)
 
-Lemma wp_if' : forall b t1 t2 Q,
-  (if b then wp t1 Q else wp t2 Q) ==> wp (trm_if b t1 t2) Q.
-Proof using. intros. applys himpl_trans wp_if. case_if~. Qed.
+(* EX1! (wp_if'') *)
+(** Prove the alternative statement of rule [wp_if],
+    either from [wp_if] or directly from [triple_if]*)
 
-(** Once again, let us check that we have not lost expressive power.
-    We prove [triple_if_case] only from [wp_if] and structural properties
-    of [wp]. Observe the transitivity step. *)
-
-Lemma triple_if_case_from_wp_if : forall b t1 t2 H Q,
-  triple (if b then t1 else t2) H Q ->
-  triple (trm_if (val_bool b) t1 t2) H Q.
-Proof using.
-  introv M. rewrite wp_equiv in *. xchange M.
-  applys himpl_trans wp_if. auto.
+Lemma wp_if'' : forall b t1 t2 Q,
+  (if b then (wp t1 Q) else (wp t2 Q)) ==> wp (trm_if b t1 t2) Q.
+Proof using. 
+  (* SOLUTION *)
+  dup.
+  { (* Proof from [wp_if] *)
+    intros. applys himpl_trans wp_if. case_if~. }
+  { (* Proof from [triple_if] *)
+     intros. rewrite <- wp_equiv. applys triple_if.
+     { intros ->. rewrite~ wp_equiv. }
+     { intros ->. rewrite~ wp_equiv. } }
+  (* /SOLUTION *)
 Qed.
 
 
 (* ******************************************************* *)
-(** ** Weakest precondition for sequence and let-bindings *)
+(** ** Definition of [wp] directly from [hoare] *)
 
-(** Consider a sequence [trm_seq t1 t2]. Recall the rule [triple_seq]. *)
+(** Let's step back on our construction so far.
 
-Parameter triple_seq : forall t1 t2 H Q H1,
-  triple t1 H (fun v => H1) ->
-  triple t2 H1 Q ->
-  triple (trm_seq t1 t2) H Q.
+    1. We defined Hoare triples ([hoare]) with respect to the big-step 
+       judgment ([eval]).
 
-(** Replacing [triple t H Q] with [H ==> wp t Q] throughout the rule gives:
+    2. We defined Separation Logic triples ([triple]) in terms of 
+       Hoare triples ([hoare]), through the definition:
+       \[forall H', hoare t (H \* H') (Q \*+ H')].
+
+    3. We defined Separation Logic weakest-preconditions ([wp]) in terms 
+       of Separation Logic triples ([triple]).
+
+    Through the construction, we established in terms reasoning rules
+    for Hoare triples ([hoare]), then for Separation Logic triples
+    ([triple]), then for weakest-preconditions ([wp]).
+
+    One natural question to raise is whether there is a more direct 
+    route to deriving reasoning rules for weakest preconditions.
+    In other words, can we obtain the same end result through simpler 
+    proofs. *)
+
+(** The notion of Hoare triple is a key abstraction that enables conduction 
+    further proofs without manipulating heaps (of type [heap]) explicitly.
+    Experiments suggest that it is always beneficial to introduce the
+    Hoare logic layer.
+
+    Thus, the only question that remains is whether it would have some 
+    interest to derive the reasoning rules for weakest preconditions ([wp])
+    directly from the the reasoning rules for Hoare triples ([hoare]),
+    that is, to bypass the reasoning rules for Separation Logic triples ([triple]).
+
+    In what follows, we show that if one cares only for [wp]-style rules,
+    the route to deriving them straight from [hoare]-style rules is indeed
+    quite short. *)
+
+(** Remark: it is technically possible to bypass even the definition of
+    [triple] and specify all functions directly using the predicate [wp],
+    however, using [triple] leads to better readability of specifications,
+    thus it seems preferable to continue using that specification style.
+    (See discussion in chapter [SLFWand], appendix on "Texan triples".) *)
+
+Module WpFromHoare.
+
+(** Recall the definition of [triple] in terms of [hoare].
 
 [[
-      H ==> (wp t1) (fun v => H1) ->
-      H1 ==> (wp t2) Q ->
-      H ==> wp (trm_seq t1 t2) Q.
+    Definition triple (t:trm) (H:hprop) (Q:val->hprop) : Prop :=
+      forall (H':hprop), hoare t (H \* H') (Q \*+ H').
 ]]
-    This entailment holds for any [H] and [H1]. Let us specialize it to
-    [H1 := (wp t2) Q] and [H := (wp t1) (fun v => (wp t2) Q)].
-    This leads us to the wp-style reasoning rule for sequences.
-    Again, we provide a direct proof from [hoare] triples. *)
+
+    In what follows, we conduct the proofs by assuming a concrete definition 
+    for [wp], namely [wp_high], which lends itself better to automated proofs. *)
+
+Definition wp (t:trm) := fun (Q:val->hprop) =>
+  \exists H, H \* \[triple t H Q].
+
+(** First, we check the equivalence between [triple t H Q] and [H ==> wp t Q].
+    This proof is the same as [wp_equiv_wp] from the module [WpHighLevel] 
+    given earlier in this chapter. *)
+
+Lemma wp_equiv : forall t H Q,
+  (triple t H Q) <-> (H ==> wp t Q).
+Proof using.
+  unfold wp. iff M.
+  { xsimpl~ H. }
+  { applys~ triple_conseq Q M.
+    applys triple_hexists. intros H'.
+    rewrite hstar_comm. applys~ triple_hpure. }
+Qed.
+
+(** Second, we prove the consequence-frame rule associated with [wp].
+    It is the only structural rule that is needed for weakest preconditions. *)
+
+Lemma wp_conseq_frame : forall t H Q1 Q2,
+  Q1 \*+ H ===> Q2 ->
+  (wp t Q1) \* H ==> (wp t Q2).
+
+(** The proof leverages the consequence rule for [hoare] triples,
+    and the frame property comes from the [forall H'] quantification
+    baked in the definition of [triple]. *)
+
+Proof using.
+  introv M. unfold wp. xpull ;=> H' N. xsimpl (H' \* H).
+  unfolds triple. intros H''. specializes N (H \* H'').
+  applys hoare_conseq N. { xsimpl. } { xchange M. }
+Qed.
+
+(** Third and last, we establish reasoning rules for terms in [wp]-style
+    directly from the corresponding rules for [hoare] triples.
+
+    The proof details are beyond the scope of this course. 
+    The point here is to show that the proofs are fairly concise. *)
+
+Lemma wp_val : forall v Q,
+  Q v ==> wp (trm_val v) Q.
+Proof using. intros. unfold wp. xsimpl. intros H'. applys hoare_val. xsimpl. Qed.
+
+Lemma wp_fun : forall x t Q,
+  Q (val_fun x t) ==> wp (trm_fun x t) Q.
+Proof using. intros. unfold wp. xsimpl. intros H'. applys hoare_fun. xsimpl. Qed.
+
+Lemma wp_fix : forall f x t Q,
+  Q (val_fix f x t) ==> wp (trm_fix f x t) Q.
+Proof using. intros. unfold wp. xsimpl. intros H'. applys hoare_fix. xsimpl. Qed.
+
+Lemma wp_if : forall b t1 t2 Q,
+  wp (if b then t1 else t2) Q ==> wp (trm_if b t1 t2) Q.
+Proof using.
+  intros. unfold wp. xsimpl. intros H M H'.
+  applys hoare_if_case. applys M.
+Qed.
 
 Lemma wp_seq : forall t1 t2 Q,
   wp t1 (fun r => wp t2 Q) ==> wp (trm_seq t1 t2) Q.
 Proof using.
-  intros. rewrite wp_def. xsimpl. intros H' M1.
-  rewrite wp_def. xsimpl. intros H''.
-  applys hoare_seq. applys (rm M1). rewrite wp_def.
-  repeat rewrite hstar_hexists. applys hoare_hexists; intros H'''.
-  rewrite (hstar_comm H'''); repeat rewrite hstar_assoc.
-  applys hoare_hpure; intros M2. applys hoare_conseq M2; xsimpl.
+  intros. unfold wp. xsimpl. intros H' M1. intros H''. applys hoare_seq.
+  { applys M1. }
+  { repeat rewrite hstar_hexists. applys hoare_hexists; intros H'''.
+    rewrite (hstar_comm H'''). repeat rewrite hstar_assoc.
+    applys hoare_hpure. intros M2. applys hoare_conseq M2. xsimpl. xsimpl. }
 Qed.
-
-(* EX2! (triple_seq_from_wp_seq) *)
-(** Once again, let us check that we have not lost expressive power.
-    Prove [triple_seq] only from [wp_seq] and structural properties
-    of [wp]. *)
-
-Lemma triple_seq_from_wp_seq : forall t1 t2 H Q H1,
-  triple t1 H (fun v => H1) ->
-  triple t2 H1 Q ->
-  triple (trm_seq t1 t2) H Q.
-Proof using.
-(* SOLUTION *)
-  introv M1 M2. rewrite wp_equiv in *. xchange M1.
-  applys himpl_trans wp_seq. applys wp_conseq. intros _. applys M2.
-(* /SOLUTION *)
-Qed.
-
-(** The rule of [trm_let x t1 t2] is very similar, the main difference
-    being the substitution on [t2]. *)
 
 Lemma wp_let : forall x t1 t2 Q,
   wp t1 (fun v => wp (subst x v t2) Q) ==> wp (trm_let x t1 t2) Q.
 Proof using.
-  intros. rewrite wp_def. xsimpl. intros H' M1.
-  rewrite wp_def. xsimpl. intros H''.
-  applys hoare_let. applys (rm M1). intros v. simpl. rewrite wp_def.
-  repeat rewrite hstar_hexists. applys hoare_hexists; intros H'''.
-  rewrite (hstar_comm H'''); repeat rewrite hstar_assoc.
-  applys hoare_hpure; intros M2. applys hoare_conseq M2; xsimpl.
+  intros. unfold wp. xsimpl. intros H' M1. intros H''. applys hoare_let.
+  { applys M1. }
+  { intros v. simpl. repeat rewrite hstar_hexists. applys hoare_hexists. intros H'''.
+    rewrite (hstar_comm H'''). repeat rewrite hstar_assoc.
+    applys hoare_hpure. intros M2. applys hoare_conseq M2. xsimpl. xsimpl. }
 Qed.
-
-
-(* ******************************************************* *)
-(** ** Weakest precondition for applications *)
-
-(** Recall the rule [triple_app_fun]. *)
-
-Parameter triple_app_fun : forall x v1 v2 t1 H Q,
-  v1 = val_fun x t1 ->
-  triple (subst x v2 t1) H Q ->
-  triple (trm_app v1 v2) H Q.
-
-(** The corresponding wp-style rule is stated and proved next. *)
 
 Lemma wp_app_fun : forall x v1 v2 t1 Q,
   v1 = val_fun x t1 ->
   wp (subst x v2 t1) Q ==> wp (trm_app v1 v2) Q.
 Proof using.
-  introv EQ1. repeat rewrite wp_def. xsimpl. intros.
-  applys* hoare_app_fun.
+  introv EQ1. unfold wp. xsimpl. intros H' M. intros H''. applys* hoare_app_fun.
 Qed.
-
-(** Similarly, the weakest-precondition rule for recursive function
-    is stated and proved next. *)
 
 Lemma wp_app_fix : forall f x v1 v2 t1 Q,
   v1 = val_fix f x t1 ->
   wp (subst x v2 (subst f v1 t1)) Q ==> wp (trm_app v1 v2) Q.
 Proof using.
-  introv EQ1. repeat rewrite wp_def. xsimpl. intros.
-  applys* hoare_app_fix.
+  introv EQ1. unfold wp. xsimpl. intros H' M. intros H''. applys* hoare_app_fix.
 Qed.
 
-
-(* ####################################################### *)
-(** * Bonus: Texan triples *)
-
-(* ******************************************************* *)
-(** ** Texan triples on a simple example *)
-
-(** In this section, we show that specification triples can be presented
-    in a different (yet equivalent) style using weakest preconditions. *)
-
-(** Consider for example the specification triple for allocation. *)
-
-Parameter triple_ref : forall v,
-  triple (val_ref v)
-    \[]
-    (fun r => \exists (l:loc), \[r = val_loc l] \* l ~~~> v).
-
-(** This specification can be equivalently reformulated in the form: *)
-
-Parameter wp_ref : forall Q v,
-  \[] \* (\forall l, l ~~~> v \-* Q (val_loc l)) ==> wp (val_ref v) Q.
-
-(** Above, we purposely left the empty heap predicate to the front to
-    indicate where the precondition, if it were not empty, would go in
-    the reformulation. *)
-
-(** In what follows, we describe the chain of transformation that can take us
-    from the triple form to the wp form, and establish the reciprocal.
-    We then formalize the general pattern for translating a triple
-    into a "texan triple" (i.e., the wp-based specification). *)
-
-(** By replacing [triple t H Q] with [H ==> wp t Q], the specification
-    gets reformulated as: *)
-
-Lemma wp_ref_0 : forall v,
-  \[] ==> wp (val_ref v) (fun r => \exists l, \[r = val_loc l] \* l ~~~> v).
-Proof using. intros. rewrite <- wp_equiv. applys triple_ref. Qed.
-
-(** The statement can be reformulated with the aim of making the RHS of the
-    form [wp (val_ref v) Q] for an abstract [Q]. *)
-
-Lemma wp_ref_1 : forall Q v,
-  ((fun r => \exists l, \[r = val_loc l] \* l ~~~> v) \--* Q) ==> wp (val_ref v) Q.
-Proof using. intros. xchange (wp_ref_0 v). applys wp_ramified_frame. Qed.
-
-(** This statement can be further reformulated by quantifying [r] with a [\forall],
-    which essentially amounts to unfolding the definition of [\--*]. *)
-
-Lemma wp_ref_2 : forall Q v,
-  (\forall r, (\exists l, \[r = val_loc l] \* l ~~~> v) \-* Q r) ==> wp (val_ref v) Q.
-Proof using. intros. applys himpl_trans wp_ref_1. xsimpl. Qed.
-
-(** The point is that now we may eliminate [r]: *)
-
-Lemma wp_ref_3 : forall Q v,
-  (\forall l, l ~~~> v \-* Q (val_loc l)) ==> wp (val_ref v) Q.
-Proof using.
-  intros. applys himpl_trans wp_ref_2.
-  xsimpl. intros ? l ->. xchange (hforall_specialize l).
-Qed.
-
-
-(* ------------------------------------------------------- *)
-(** *** 2. The general pattern *)
-
-(** In practice, specification triples can (pretty much) all be casted
-    in the form: [triple t H (fun r => exists x1 x2, \[r = v] \* H'].
-    The value [v] may depend on the [xi].
-    The heap predicate [H'] may depend on [r] and the [xi].
-    The number of existentials [xi] may vary, possibly be zero.
-    The equality \[r = v] may degenerate to \[r = r] if no pure fact
-    is needed about [r].
-
-    A triple of the above form may be reformulated as:
-    [(\forall x1 x2, H \-* Q v) ==> wp t Q].
-
-    We next formalize this result for the case of a single [xi] variable,
-    making it explicit that [H] and [v] may depend on it. *)
-
-Lemma texan_triple_equiv : forall t H A (Hof:val->A->hprop) (vof:A->val),
-      (triple t H (fun r => \exists x, \[r = vof x] \* Hof r x))
-  <-> (forall Q, H \* (\forall x, Hof (vof x) x \-* Q (vof x)) ==> wp t Q).
-Proof using.
-  intros. rewrite wp_equiv. iff M.
-  { intros Q. xchange M. applys wp_ramified_trans.
-    xsimpl. intros r x ->. xchanges (hforall_specialize x). }
-  { applys himpl_trans M. xsimpl~. }
-Qed.
-
-
-(* ------------------------------------------------------- *)
-(** *** 3. Exercise *)
-
-(** Recall the function [incr] and its specification. *)
-
-Parameter incr : val. (** Code omitted, may be found in [SLFHprop.v]. *)
-
-Parameter triple_incr : forall (p:loc) (n:int),
-  triple (trm_app incr p)
-    (p ~~~> n)
-    (fun v => \[v = val_unit] \* (p ~~~> (n+1))).
-
-(* EX2! (wp_incr) *)
-(** State a Texan triple for [incr] as a lemma [wp_incr],
-    then prove this lemma from [triple_incr].
-
-    Hint: the proof is a bit easier by first turning the [wp] into a [triple]
-    and then reasoning about triples, compared than working on the [wp] form. *)
-
-(* SOLUTION *)
-Lemma wp_incr : forall (p:loc) (n:int) Q,
-  (p ~~~> n) \* (p ~~~> (n+1) \-* Q val_unit) ==> wp (trm_app incr p) Q.
-Proof using.
-  intros. rewrite <- wp_equiv. applys triple_conseq_frame.
-  { applys triple_incr. } { xsimpl. } { xsimpl ;=> ? ->. auto. }
-Qed.
-(* /SOLUTION *)
-
-
-
-(* ******************************************************* *)
-(** ** Chapter's notes *)
-
-(** Texan triples are used in Iris. *)
+End WpFromHoare.
 
